
Answer for question 3 in Exercise 7
=====================================
As k increases, the value of f will become 1.


Answer for question 4 in Exercise 7
=====================================
Luckily, the only change made on the function in every iteration is a multiplication. So, if we are able to get this term that gets multiplied as a function of f, we might be able to just multiply it using the new value of "o" and use this updated product term to find the next f.


Answer for question 5 in Exercise 7
=====================================
Another way to implement it would be using recursiveness. Pretty much applying what I described in question 4, but calling the function every time we want to update the product term to find the new f.
